

# Fourier Analysis Notes (Stein-Shakarchi)

Prashant Rao

**Theorem 1.** Let  $u : \mathbb{R}^2 \rightarrow \mathbb{R}$  be twice differentiable in both variables, and define a change of variables via polar coordinates from  $(x, y) \in \mathbb{R}^2$  to  $(r, \theta) \in \mathbb{R}_+ \times [0, 2\pi)$ :

$$x = r \cos \theta \qquad y = r \sin \theta$$

Then, we can write:

$$\Delta u = \frac{\partial^2 u}{\partial r^2} + \frac{\partial^2 u}{\partial \theta^2} \frac{1}{r^2} + \frac{\partial u}{\partial r} \frac{1}{r}$$

*Proof:* First note:

$$\begin{aligned} r^2 &= x^2 + y^2 \\ \implies \frac{\partial r}{\partial x} &= \frac{x}{r} = \cos \theta \end{aligned}$$

and similarly:

$$\frac{\partial r}{\partial y} = \frac{y}{r} = \sin \theta$$

for  $\theta$  we have:

$$\begin{aligned} \theta &= \arctan \frac{y}{x} \\ \implies \frac{\partial \theta}{\partial x} &= \frac{1}{1 + \left(\frac{y}{x}\right)^2} \cdot -\frac{y}{x^2} = -\frac{y}{x^2 + y^2} = -\frac{\sin \theta}{r} \\ \frac{\partial \theta}{\partial y} &= \frac{1}{1 + \left(\frac{y}{x}\right)^2} \cdot \frac{1}{x} = \frac{x}{x^2 + y^2} = \frac{\cos \theta}{r} \end{aligned}$$

Thus for any function  $f$  of  $(x, y) \in \mathbb{R}^2$ , we have:

$$\begin{aligned} \frac{\partial f}{\partial x} &= \frac{\partial f}{\partial r} \frac{\partial r}{\partial x} + \frac{\partial f}{\partial \theta} \frac{\partial \theta}{\partial x} = \frac{\partial f}{\partial r} \cos \theta - \frac{\partial f}{\partial \theta} \frac{\sin \theta}{r} \\ \frac{\partial f}{\partial y} &= \frac{\partial f}{\partial r} \frac{\partial r}{\partial y} + \frac{\partial f}{\partial \theta} \frac{\partial \theta}{\partial y} = \frac{\partial f}{\partial r} \sin \theta + \frac{\partial f}{\partial \theta} \frac{\cos \theta}{r} \end{aligned}$$

Hence we can evaluate:

$$\frac{\partial u}{\partial x} = \frac{\partial u}{\partial r} \cos \theta - \frac{\partial u}{\partial \theta} \frac{\sin \theta}{r}$$

so:

$$\begin{aligned} \frac{\partial^2 u}{\partial x^2} &= \frac{\partial u_x}{\partial r} \cos \theta - \frac{\partial u_x}{\partial \theta} \frac{\sin \theta}{r} \\ &= \left( \frac{\partial^2 u}{\partial r^2} \cos \theta - \frac{\partial^2 u}{\partial r \partial \theta} \frac{\sin \theta}{r} + \frac{\partial u}{\partial \theta} \frac{\sin \theta}{r^2} \right) \cos \theta \\ &\quad - \left( \frac{\partial^2 u}{\partial r \partial \theta} \cos \theta - \frac{\partial u}{\partial r} \sin \theta - \frac{\partial^2 u}{\partial \theta^2} \frac{\sin \theta}{r} - \frac{\partial u}{\partial \theta} \frac{\cos \theta}{r} \right) \frac{\sin \theta}{r} \\ &= \frac{\partial^2 u}{\partial r^2} \cos^2 \theta + \frac{\partial^2 u}{\partial \theta^2} \frac{\sin^2 \theta}{r^2} - 2 \frac{\partial^2 u}{\partial r \partial \theta} \frac{\sin \theta \cos \theta}{r} + \frac{\partial u}{\partial r} \frac{\sin^2 \theta}{r} + 2 \frac{\partial u}{\partial \theta} \frac{\sin \theta \cos \theta}{r^2} \end{aligned}$$

and similarly:

$$\begin{aligned}
\frac{\partial u}{\partial y} &= \frac{\partial u}{\partial r} \sin \theta + \frac{\partial u}{\partial \theta} \frac{\cos \theta}{r} \\
\Rightarrow \frac{\partial^2 u}{\partial y^2} &= \frac{\partial^2 u}{\partial r^2} \sin \theta + \frac{\partial^2 u}{\partial \theta^2} \frac{\cos \theta}{r} \\
&= \left( \frac{\partial^2 u}{\partial r^2} \sin \theta + \frac{\partial^2 u}{\partial r \partial \theta} \frac{\cos \theta}{r} - \frac{\partial u}{\partial \theta} \frac{\cos \theta}{r^2} \right) \sin \theta \\
&\quad + \left( \frac{\partial^2 u}{\partial \theta \partial r} \sin \theta + \frac{\partial u}{\partial r} \cos \theta + \frac{\partial^2 u}{\partial \theta^2} \frac{\cos \theta}{r} - \frac{\partial u}{\partial \theta} \frac{\sin \theta}{r} \right) \frac{\cos \theta}{r} \\
&= \frac{\partial^2 u}{\partial r^2} \sin^2 \theta + \frac{\partial^2 u}{\partial \theta^2} \frac{\cos^2 \theta}{r^2} + 2 \frac{\partial^2 u}{\partial r \partial \theta} \frac{\cos \theta \sin \theta}{r} + \frac{\partial u}{\partial r} \frac{\cos^2 \theta}{r} - 2 \frac{\partial u}{\partial \theta} \frac{\sin \theta \cos \theta}{r^2}
\end{aligned}$$

hence:

$$\Delta u = \frac{\partial^2 u}{\partial x^2} + \frac{\partial^2 u}{\partial y^2} = \frac{\partial^2 u}{\partial r^2} + \frac{\partial^2 u}{\partial \theta^2} \frac{1}{r^2} + \frac{\partial u}{\partial r} \frac{1}{r}$$

□

**Theorem 2** (Stein-Shakarchi Theorem 2.1). *Suppose  $f$  is an integrable function on the circle with all Fourier coefficients equal to zero. Then  $f(\theta_0) = 0$  whenever  $f$  is continuous at  $\theta_0$ .*

*Proof.* First let us show that without loss of generality we can assume  $\theta_0 = 0$ . To see this, define  $g(x) = f(x + \theta_0)$  where  $f$  is considered to be periodic on  $\mathbb{R}$ . Then for all  $n \in \mathbb{Z}$ :

$$\left| \int_{-\pi}^{\pi} g(x) e^{inx} dx \right| = \left| e^{-in\theta_0} \int_{-\pi+\theta_0}^{\pi+\theta_0} f(x) e^{inx} dx \right| = \left| \int_{-\pi}^{\pi} f(x) e^{inx} dx \right|$$

Thus the Fourier coefficients of  $g$  are equal to the Fourier coefficients of  $f$  in modulus, meaning they are all 0 if and only if the coefficients of  $f$  are all 0 (which is an assumption of the theorem). If we can prove  $g(0) = 0$  when the coefficients of  $g$  are all 0, then we know  $f(\theta_0) = g(0) = 0$  too.

It should also be obvious we can assume  $f(0) > 0$  (if not we can just replace  $f$  with  $-f$  in the following).

Now, choose  $\delta \in (0, \pi/2]$  such that  $f > f(0)/2$  on  $(-\delta, \delta)$ . This is possible because  $f$  is continuous so we can always find a ball around 0 where  $f$  is sufficiently close to  $f(0)$ .

Then we can define  $p(\theta) := \varepsilon + \cos \theta$  where we can choose  $\varepsilon > 0$  sufficiently small such that  $|p(\theta)| < 1 - \varepsilon/2$  whenever  $|\theta| \in [\delta, \pi]$ . We can think of this like shifting up so instead of  $p(\delta) \in (0, 1)$  and  $p(\pi) = -1$  we increase  $p$  a bit so that  $p(\delta) < 1$  still but  $p(\pi) > -1$ .

Lastly we can choose  $\eta \in (0, \delta)$  so that  $p(\theta) \geq 1 + \varepsilon/2$  for  $|\theta| < \eta$ . This works because we already shifted up  $\cos$  by  $\varepsilon$ .

We can now let  $p_k(\theta) = [p(\theta)]^k$ . Since this is a trigonometric polynomial we see for all  $k \in \mathbb{N}$ :

$$\int_{-\pi}^{\pi} f(\theta) p_k(\theta) d\theta = 0$$

Also we can see:

$$\left| \int_{B_\delta(0)^c} f(\theta) p_k(\theta) d\theta \right| \leq 2\pi (1 - \varepsilon/2)^k \sup |f|$$

and:

$$\int_{B_\delta(0) \cap B_\eta(0)^c} f(\theta) p_k(\theta) d\theta \geq 0$$

since  $f \geq f(0)/2 > 0$  and  $p > 0$  on  $B_\delta(0)$ . Finally:

$$\int_{B_\eta(0)} f(\theta) p_k(\theta) d\theta \geq \eta (1 + \varepsilon/2)^k f(0)$$

Since this grows unboundedly in  $k$ , we can see:

$$\int_{-\pi}^{\pi} f(\theta) p_k(\theta) d\theta \xrightarrow{k \rightarrow \infty} \infty$$

which is a contradiction since those integrals must all be 0.

We can generalise the proof to complex valued  $f$  by writing  $f = u + iv$ . This lets us recover  $u$  and  $v$  from  $f$  and  $\bar{f}$ . Using the fact that the  $n$ -th Fourier coefficient of  $f$  is the  $-n$ -th coefficient of its conjugate, we can show if all the Fourier coefficients of  $f$  are zero then all the Fourier coefficients of  $u$  and  $v$  are zero, and we are done.  $\square$

From this we can see if  $f$  is continuous on the circle and all of its Fourier coefficients are zero then  $f$  is zero identically.

**Theorem 3** (Convergence of Cesaro sums). *Suppose a sequence  $z_n$  converges to  $A$ . Then the Cesaro sums of  $z_n$  also converge to  $A$*

*Proof.* Without loss of generality assume  $A = 0$ . If not define  $y_n = z_n - A$ , and notice that  $y_n \rightarrow 0$  and

$$\frac{\sum_{i=1}^N y_i}{N} = \frac{\sum_{i=1}^N (z_i - A)}{N} = \frac{\sum_{i=1}^N z_i}{N} - A$$

meaning if we show the Cesaro sums of  $y_n$  converge to zero, we show the Cesaro sums of  $z_n$  converge to  $A$ . Let  $\varepsilon > 0$  be given and choose  $M > 0$  such that  $|y_m| < \varepsilon/2$  for  $m > M$ . Also note that we know  $y_n$  are bounded since they are convergent.

For any  $n > M$ :

$$\begin{aligned} \left| \frac{1}{n} \sum_{i=1}^n y_i \right| &\leq \frac{1}{n} \sum_{i=1}^M |y_i| + \frac{1}{n} \sum_{i=M+1}^n |y_i| \\ &\leq \frac{M}{n} \sup_{i \in \mathbb{N}} |y_i| + \left(1 - \frac{M}{n}\right) \frac{\varepsilon}{2} \xrightarrow{n \rightarrow \infty} \frac{\varepsilon}{2} \end{aligned}$$

Hence there exists some  $N > M$  such that for all  $n > N$  we have:

$$\left| \frac{1}{n} \sum_{i=1}^n y_i \right| < \varepsilon$$

$\square$

By linearity of convolution we know the Cesaro means of the Fourier series are given by convolution with Fejer kernels:

$$F_n = \frac{1}{n} \sum_{i=0}^{n-1} D_i$$

We can define a notion of a good kernel:

**Definition 1** (Good kernel). *A family of kernels  $(K_n)$  is a family of good kernels if it satisfies:*

1. For all  $n \in \mathbb{N}$

$$\frac{1}{2\pi} \int_{-\pi}^{\pi} K_n(t) dt = 1$$

2. There exists  $M > 0$  such that for all  $n \in \mathbb{N}$

$$\int_{-\pi}^{\pi} |K_n(t)| dt \leq M$$

3. For all  $\delta > 0$  we have

$$\lim_{n \rightarrow \infty} \int_{B_\delta(0)^c} |K_n(t)| dt = 0$$

These are important because they approximate the identity in convolution.

**Theorem 4.** If  $(K_n)$  is a family of good kernels, and  $f$  is continuous at  $x$ , we have  $K_n * f(x) \rightarrow f(x)$  as  $n \rightarrow \infty$ . Furthermore, if  $f$  is uniformly continuous, then  $K_n * f \rightarrow f$  in the supremum norm.

We can directly compute the Fejer kernels and show they are good kernels.

**Theorem 5.** The Fejer kernels are good kernels.

First we will to show a brief identity for our computation:

**Lemma 1.**

$$e^{i\theta} + e^{-i\theta} - 2 = -4 \sin^2 \frac{\theta}{2}$$

*Proof:*

$$\sin^2 \frac{\theta}{2} = \left( \frac{e^{i\theta/2} - e^{-i\theta/2}}{2i} \right)^2 = -\frac{e^{i\theta} + e^{-i\theta} - 2}{4}$$

□

With this we can continue with the proof.

*Proof of theorem 5:* First we will consider the Dirichlet kernels  $D_N$ , where convolution with these kernels gives the Fourier series.

$$D_N(\theta) = \sum_{n=-N}^N e^{in\theta}$$

We know for all  $n \in \mathbb{Z}$  we have:

$$\frac{1}{2\pi} \int_{-\pi}^{\pi} e^{in\theta} d\theta = \begin{cases} 1 & \text{if } n = 0 \\ 0 & \text{otherwise} \end{cases}$$

so we have:

$$\frac{1}{2\pi} \int_{-\pi}^{\pi} D_N(\theta) d\theta = 1$$

We can compute  $D_N$  in closed form

$$\begin{aligned} D_N(\theta) &= \sum_{n=-N}^N e^{in\theta} \\ &= \sum_{n=-N}^N \cos n\theta + i \sum_{n=-N}^N \sin n\theta \end{aligned}$$

noting  $\sin n\theta = -\sin(-n\theta)$ :

$$= 1 + 2 \sum_{n=1}^N \cos n\theta$$

using that  $2 \cos u \sin v = \sin(u+v) - \sin(u-v)$ :

$$\begin{aligned}
&= 1 + \sum_{n=1}^N \frac{\sin\left(\left(n + \frac{1}{2}\right)\theta\right) - \sin\left(\left(n - \frac{1}{2}\right)\theta\right)}{\sin\left(\frac{\theta}{2}\right)} \\
&= 1 + \frac{1}{\sin\left(\frac{\theta}{2}\right)} \left( \sin\left(\frac{3}{2}\theta\right) - \sin\left(\frac{1}{2}\theta\right) + \sin\left(\frac{5}{2}\theta\right) - \sin\left(\frac{3}{2}\theta\right) + \dots \right. \\
&\quad \left. + \sin\left(\left(N + \frac{1}{2}\right)\theta\right) - \sin\left(\left(N - \frac{1}{2}\right)\theta\right) \right) \\
&= 1 + \frac{\sin\left(\left(N + \frac{1}{2}\right)\theta\right) - \sin\left(\frac{\theta}{2}\right)}{\sin\left(\frac{\theta}{2}\right)} \\
&= \frac{\sin\left(\left(N + \frac{1}{2}\right)\theta\right)}{\sin\left(\frac{\theta}{2}\right)}
\end{aligned}$$

Now we can directly compute:

$$\begin{aligned}
F_n(\theta) &= \frac{1}{n} \sum_{k=0}^{n-1} D_k(\theta) \\
&= \frac{1}{n} \sum_{k=0}^{n-1} \sum_{m=-k}^k e^{im\theta} \\
&= \frac{1}{n} \sum_{k=0}^{n-1} e^{-ik\theta} \sum_{m=-k}^k e^{i(m+k)\theta} \\
&= \frac{1}{n} \sum_{k=0}^{n-1} e^{-ik\theta} \sum_{m=0}^{2k} e^{im\theta} \\
&= \frac{1}{n} \sum_{k=0}^{n-1} \frac{e^{-ik\theta} (1 - e^{i(2k+1)\theta})}{1 - e^{i\theta}} \\
&= \frac{1}{n(1 - e^{i\theta})} \sum_{k=0}^{n-1} (e^{-ik\theta} - e^{i(k+1)\theta}) \\
&= \frac{1}{n(1 - e^{i\theta})} \left( \frac{1 - e^{-in\theta}}{1 - e^{-i\theta}} - e^{i\theta} \cdot \frac{1 - e^{in\theta}}{1 - e^{i\theta}} \right) \\
&= \frac{1}{n(1 - e^{i\theta})} \left( \frac{1 - e^{-in\theta}}{1 - e^{-i\theta}} + \frac{1 - e^{in\theta}}{1 - e^{-i\theta}} \right) \\
&= \frac{2 - e^{-in\theta} - e^{in\theta}}{n(1 - e^{i\theta})(1 - e^{-i\theta})} \\
&= \frac{2 - e^{-in\theta} - e^{in\theta}}{n(2 - e^{i\theta} - e^{-i\theta})}
\end{aligned}$$

by lemma 1:

$$= \frac{\sin^2 \frac{N\theta}{2}}{n \sin^2 \frac{\theta}{2}}$$

□